TabularTypeInterpreter/Logic/Relation.lean
@@ -2,6 +2,67 @@ import Mathlib.Logic.Relation
 
 namespace Relation
 
+inductive IndexedReflTransGen (r : α → α → Prop) : Nat → α → α → Prop where
+  | refl : IndexedReflTransGen r 0 a a
+  | tail {b c} : IndexedReflTransGen r n a b → r b c → IndexedReflTransGen r (n + 1) a c
+
+attribute [refl] IndexedReflTransGen.refl
+
+namespace IndexedReflTransGen
+
+@[trans]
+theorem trans (hab : IndexedReflTransGen r m a b) (hbc : IndexedReflTransGen r n b c)
+  : IndexedReflTransGen r (m + n) a c := by
+  induction hbc with
+  | refl => assumption
+  | tail _ hcd hac => exact hac hab |>.tail hcd
+
+instance
+  : Trans (IndexedReflTransGen r m) (IndexedReflTransGen r n) (IndexedReflTransGen r (m + n)) where
+  trans := trans
+
+theorem single (hab : r a b) : IndexedReflTransGen r 1 a b := refl.tail hab
+
+theorem head (hab : r a b) (hbc : IndexedReflTransGen r n b c)
+  : IndexedReflTransGen r (n + 1) a c := by
+  induction hbc with
+  | refl => exact refl.tail hab
+  | tail _ hcd hac => exact hac hab |>.tail hcd
+
+@[elab_as_elim]
+theorem head_induction_on {P : ∀ n : Nat, ∀ a : α, IndexedReflTransGen r n a b → Prop} {a : α}
+  (h : IndexedReflTransGen r n a b) (refl : P 0 b refl)
+  (head : ∀ {n a c} (h' : r a c) (h : IndexedReflTransGen r n c b), P n c h → P (n + 1) a (h.head h'))
+  : P n a h := by
+  induction h with
+  | refl => exact refl
+  | @tail n b c _ _ hbc ih =>
+    apply ih
+    · exact head hbc _ refl
+    · exact fun h1 h2 ↦ head h1 (h2.tail hbc)
+
+theorem cases_head (h : IndexedReflTransGen r n a b)
+  : (n = 0 ∧ a = b) ∨ ∃ m c, n = m + 1 ∧ r a c ∧ IndexedReflTransGen r m c b := by
+  induction h using Relation.IndexedReflTransGen.head_induction_on
+  · exact .inl ⟨rfl, rfl⟩
+  · exact .inr ⟨_, _, rfl, by assumption, by assumption⟩
+
+theorem map {r : α → α → Prop} {f : _ → _} (map_rel : ∀ {a b}, r a b → r (f a) (f b))
+  (h : IndexedReflTransGen r n a b) : IndexedReflTransGen r n (f a) (f b) := by
+  induction h with
+  | refl => rfl
+  | tail _ b'c' ih =>
+    exact ih.trans <| .single <| map_rel b'c'
+
+theorem map₂ {r : α → α → Prop} {f : _ → _ → _} (map_rel₀ : ∀ {a b c}, r a c → r (f a b) (f c b))
+  (map_rel₁ : ∀ {a b d}, r b d → r (f a b) (f a d)) (ac : IndexedReflTransGen r m a c)
+  (bd : IndexedReflTransGen r n b d) : IndexedReflTransGen r (m + n) (f a b) (f c d) := by
+  calc
+    IndexedReflTransGen r m (f a b) (f c b) := map map_rel₀ ac
+    IndexedReflTransGen r n (f c b) (f c d) := map map_rel₁ bd
+
+end IndexedReflTransGen
+
 namespace ReflTransGen
 
 theorem map {r : α → α → Prop} {f : _ → _} (map_rel : ∀ {a b}, r a b → r (f a) (f b))
